\documentclass[11pt, leqno]{article}

%{{{ preamble

\def\doc{The n-Pendulum Problem}
 \def\course{self-study}
\def\abbrev{n-pendulum}
\def\name{A. Mayorov}

\input{preamble_ru_homework}

% fix some spacing
% http://tex.stackexchange.com/questions/22119/how-can-i-change-the-spacing-before-theorems-with-amsthm

%\makeatletter
%\def\thm@space@setup{%
%\thm@preskip=\parskip \thm@postskip=0pt
%}

%}}}

\usepackage{tikz-qtree}
\usepackage{multirow}
\usepackage{cellspace}
\setlength{\cellspacetoplimit}{0.7em}
\setlength{\cellspacebottomlimit}{0.7em} 

\newtheorem*{note-none}{Замечание}

\usepackage{longtable}
\newcommand{\given}{\;\middle|\;}

\renewcommand{\thesection}{\Alph{section}.}

\begin{document}\thispagestyle{empty}

\begin{center}
	\textbf{\LARGE\doc}\\
	\vspace{.85em}
	\textit{\large Alex Mayorov}
\end{center}
\vspace{1em}

\section{The double pendulum}

I follow the derivation from \href{https://scipython.com/blog/the-double-pendulum/}{here}.

\begin{figure}[H]
        \centering
        \includegraphics[scale=0.6]{fig/double-pendulum-geometry}
\end{figure}

The two degrees of freedom are $\theta_1$ and $\theta_2$. Then
\begin{align*}
	x_1 &= l_1\sin\theta_1 & \dot x_1 &= l_1 \dot \theta_1 \cos\theta_1 \\
	y_1 &= -l_1 \cos\theta_1 & \dot y_1 &= l_1\dot \theta_1 \sin\theta_1\\
	x_2 &= l_1\sin\theta_1 + l_2\sin\theta_2 & \dot x_2 &= l_1 \dot \theta_1 \cos\theta_1 + l_2 \dot \theta_2 \cos\theta_2\\
	y_2 &= -l_1 \cos\theta_1 - l_2\cos\theta_2 & \dot y_2 &= l_1\dot \theta_1 \sin \theta_1 + l_2 \dot \theta_2 \sin \theta_2
.\end{align*}

Let's compute the Lagrangian, $\mathcal{L} = T - V$:
\begin{align*}
	V ={}& m_1g y_1 + m_2gy_2 \\
	={}& -m_1gl_1\cos\theta_1 - m_2g(l_1\cos\theta_1 + l_2\cos\theta_2) \\
	={}& -(m_1+m_2)gl_1\cos\theta_1-m_2gl_2\cos\theta_2 \\
	T ={}& \frac{1}{2}m_1\dot x_1^2 + \frac{1}{2}m_2\dot x_2^2 + \frac{1}{2}m_1\dot y_1^2 + \frac{1}{2}m_2\dot y_2^2\\
	={}& \frac{1}{2}m_1l_1^2\dot \theta_1^2 + \frac{1}{2}m_2(l_2^2\dot\theta_1^2 + 2l_1l_2\dot\theta_1\dot\theta_2 \cos(\theta_1-\theta_2) + l_2^2\dot\theta_2^2) \\
	={}& \frac{1}{2}(m_1 + m_2)l_1^2\dot \theta_1^2 + \frac{1}{2}m_2l_2^2\dot\theta_2^2 + m_2l_1l_2\dot\theta_1\dot\theta_2\cos(\theta_1-\theta_2) \\
	\mathcal{L} ={}&   \frac{1}{2}(m_1 + m_2)l_1^2\dot \theta_1^2 + \frac{1}{2}m_2l_2^2\dot\theta_2^2 + m_2l_1l_2\dot\theta_1\dot\theta_2\cos(\theta_1-\theta_2) \\
		       &+(m_1+m_2)gl_1\cos\theta_1+m_2gl_2\cos\theta_2
.\end{align*}

We apply the Euler-Lagrange equations, which are:
\begin{equation*}
	\frac{d}{dt}\left( \frac{\partial \mathcal{L}}{\partial \dot q_i} \right)  - \frac{\partial \mathcal{L}}{\partial q_i} = 0\qquad \text{for } q_i = \theta_1, \theta_2 
.\end{equation*}

Therefore,
\begin{align*}
	\frac{\partial \mathcal{L}}{\partial \dot \theta_1} ={}& (m_1 + m_2) l_1^2 \dot \theta_1 + m_2l_1l_2\dot\theta_2\cos(\theta_1 - \theta_2)\\
	\frac{\partial \mathcal{L}}{\partial \theta_1} ={}& -m_2l_1l_2\dot \theta_1\dot \theta_2 \sin(\theta_1-\theta_2) -(m_1+m_2)l_1g \sin\theta_1
\end{align*}
and
\begin{align*}
	&
	\!\begin{multlined}[b]
	 \implies(m_1+m_2)l_1^2\ddot \theta_1 + m_2l_1l_2\ddot \theta_2\cos(\theta_1-\theta_2) - m_2l_1l_2\dot \theta_2\sin(\theta_1-\theta_2)(\dot \theta_1-\dot \theta_2) \\
	= -m_2l_1l_2\dot \theta_1\dot \theta_2\sin(\theta_1-\theta_2) - (m_1+m_2)l_1g\sin\theta_1
	\end{multlined}\\
	&\implies
	(m_1+m_2)l_1\ddot \theta_1 + m_2l_2\ddot \theta_2\cos(\theta_1-\theta_2) + m_2l_2\dot \theta_2^2 \sin(\theta_1-\theta_2) + (m_1+m_2)g\sin\theta_1 = 0
.\end{align*}

Again,
\begin{align*}
	\frac{\partial \mathcal{L}}{\partial \dot \theta_2} ={}& m_2l_2^2\dot \theta_2 + m_2l_1l_2\dot \theta_1\cos(\theta_1-\theta_2) \\
	\frac{\partial \mathcal{L}}{\partial \theta_2} ={}& m_2l_1l_2\dot \theta_1 \dot \theta_2 \sin(\theta_1-\theta_2) - m_2gl_2\sin\theta_2 \\
\end{align*}
and
\begin{align*}
	&\implies m_2l_2\ddot \theta_2 + m_2l_1\ddot \theta_1 \cos(\theta_1-\theta_2) -m_2l_1\dot \theta_1 \sin(\theta_1-\theta_2)(\dot \theta_1 - \dot \theta_2) = m_2l_1\dot \theta_1\dot \theta_2\sin(\theta_1-\theta_2) - m_2g\sin\theta_2\\
	&\implies m_2l_2 \ddot{\theta_2} + m_2l_1 \ddot{\theta_1}\cos(\theta_1-\theta_2)-m_2l_1 \dot{\theta_1^2}\sin(\theta_1-\theta_2) + m_2g\sin\theta_2 = 0
.\end{align*}

Let's introduce $z_1 = \dot{\theta_1}, \dot{z_1} = \ddot{\theta_1}, z_2= \dot{\theta_2}, \dot{z_2} = \ddot{\theta_2}$. This implies

\begin{gather*}
	\begin{cases}
		(m_1+m_2)l_1 \dot{z_1} + m_2l_2 \dot{z_2} \cos(\theta_1-\theta_2) + m_2l_2 z_2^2\sin(\theta_1-\theta_2) + (m_1+m_2)g \sin\theta_1 = 0\\
		m_2l_2 \dot{z_2} + m_2l_1 \dot{z_1}\cos(\theta_1-\theta_2) - m_2l_1z_1^2\sin(\theta_1-\theta_2) + m_2g\sin \theta_2 = 0
	\end{cases}\\ \\
	\begin{cases}
		\begin{split}
			(m_1+m_2)l_1 \dot{z_1} - m_2l_1 \dot{z_1}\cos^2(\theta_1-\theta_2) + m_2l_2 z_2^2\sin(\theta_1-\theta_2) + (m_1+m_2)g\sin\theta_1\\ + m_2l_1z_1^2 \sin(\theta_1-\theta_2)\cos(\theta_1-\theta_2) - m_2g\sin\theta_2\cos(\theta_1-\theta_2) = 0
		\end{split}\\
		\begin{split}
			m_2l_2 \dot{z_2}(m_1+m_2)-m_2l_1z_1^2\sin(\theta_1-\theta_2) (m_1+m_2) +m_2g\sin\theta_2(m_1+m_2) - m_2^2l_2 \dot{z_2} \cos^2(\theta_1-\theta_2) \\ - m_2^2l_2z_2^2\sin(\theta_1-\theta_2) \cos(\theta_1-\theta_2) - (m_1+m_2)m_2g\sin\theta_1\cos(\theta_1-\theta_2) = 0
		\end{split}
	\end{cases}\\ \\
	\begin{cases}
		\dot{z_1} = \frac{m_2g\sin\theta_2\cos(\theta_1-\theta_2) - m_2\sin(\theta_1-\theta_2)[l_1z_1^2\cos(\theta_1-\theta_2) + l_2z_2^2] - (m_1 + m_2)g\sin\theta_1}{l_1[m_1 + m_2\sin^2(\theta_1-\theta_2)]} \\
		\dot{z_2} = \frac{(m_1+m_2)[l_1z_1^2\sin(\theta_1-\theta_2) - g\sin\theta_2  + g\sin\theta_1 \cos(\theta_1-\theta_2)] + m_2l_2z_2^2\sin(\theta_1-\theta_2)\cos(\theta_1-\theta_2)}{l_2[m_1 + m_2\sin^2(\theta_1-\theta_2)]}
	\end{cases}
.\end{gather*}

This forms a system of four first-order ODE in $\dot{z_1}, \dot{\theta_1}, \dot{z_2}, \dot{\theta_2}$ that we can solve numerically, using the Euler or Runge-Kutta method.

\pagebreak
\tableofcontents{}

\end{document}
